add low-level spec of montgomery ladder for exp

code/bignum/Hacl.Spec.Bignum.Exponentiation.fst
@@ -13,6 +13,7 @@ open Hacl.Spec.Bignum.ModInv64
 
 module BL = Hacl.Spec.Exponentiation.Lemmas
 module M = Hacl.Spec.Montgomery.Lemmas
+module L = Hacl.Spec.Bignum.Lib // for cswap
 
 #reset-options "--z3rlimit 50 --fuel 0 --ifuel 0"
 
@@ -28,7 +29,6 @@ val bn_mod_exp_f:
   tuple2 (lbignum nLen) (lbignum nLen)
 
 let bn_mod_exp_f #nLen n mu bBits bLen b i (aM, accM) =
-  [@inline_let]
   let is_bit_set = FStar.UInt64.(Lib.RawIntTypes.u64_to_UInt64 (bn_get_ith_bit #bLen b i) =^ 1uL) in
   let accM = if is_bit_set then mont_mul n mu aM accM else accM in // acc = (acc * a) % n
   let aM = mont_sqr n mu aM in // a = (a * a) % n
@@ -54,6 +54,7 @@ let bn_mod_exp_mont modBits nLen n a acc bBits b =
   let accM = to_mont n mu r2 acc in
   let (aM, accM) = repeati bBits (bn_mod_exp_f #nLen n mu bBits bLen b) (aM, accM) in
   from_mont n mu accM
+
 
 let bn_mod_exp modBits nLen n a bBits b =
   let acc = bn_from_uint nLen (u64 1) in
@@ -199,3 +200,219 @@ let bn_mod_exp_lemma modBits nLen n a bBits b =
   let d, k = M.eea_pow2_odd (64 * nLen) (bn_v n) in
   M.mont_preconditions nLen (bn_v n) (v mu);
   BL.mod_exp_mont_ll_lemma nLen (bn_v n) d (v mu) (bn_v a) bBits (bn_v b)
+
+///
+///  Montgomery ladder for exponentiation
+///
+
+val bn_mod_exp_mont_ladder_f:
+    #nLen:size_pos{nLen + nLen <= max_size_t}
+  -> n:lbignum nLen
+  -> mu:uint64
+  -> bBits:size_pos
+  -> bLen:size_nat{bLen == blocks bBits 64}
+  -> b:lbignum bLen
+  -> i:nat{i < bBits}
+  -> rM0_rM1_privbit: tuple3 (lbignum nLen) (lbignum nLen) uint64 ->
+  tuple3 (lbignum nLen) (lbignum nLen) uint64
+
+let bn_mod_exp_mont_ladder_f #nLen n mu bBits bLen b i (rM0, rM1, privbit) =
+  let bit = bn_get_ith_bit #bLen b (bBits - i - 1) in
+  let sw = bit ^. privbit in
+  let rM0, rM1 = L.cswap2 sw rM0 rM1 in
+  let rM0' = mont_sqr n mu rM0 in // rM0 * rM0 % n
+  let rM1' = mont_mul n mu rM1 rM0 in // rM1 * rM0 % n
+  (rM0', rM1', bit)
+
+
+val bn_mod_exp_mont_ladder_:
+    modBits:size_pos
+  -> nLen:size_pos{128 * nLen <= max_size_t}
+  -> n:lbignum nLen{nLen == blocks modBits 64}
+  -> a:lbignum nLen
+  -> acc:lbignum nLen
+  -> bBits:size_pos
+  -> b:lbignum (blocks bBits 64) ->
+  lbignum nLen
+
+let bn_mod_exp_mont_ladder_ modBits nLen n a one bBits b =
+  let bLen = blocks bBits 64 in
+  let mu = mod_inv_u64 n.[0] in
+
+  let r2 = precomp_r2_mod_n #nLen modBits n in
+  let rM0 = to_mont n mu r2 one in
+  let rM1 = to_mont n mu r2 a in
+  let sw = u64 0 in
+  let (rM0', rM1', sw') = repeati bBits (bn_mod_exp_mont_ladder_f #nLen n mu bBits bLen b) (rM0, rM1, sw) in
+  let (rM0', rM1') = L.cswap2 sw' rM0' rM1' in
+  from_mont n mu rM0'
+
+
+let bn_mod_exp_mont_ladder modBits nLen n a bBits b =
+  let acc = bn_from_uint nLen (u64 1) in
+  bn_mod_exp_mont_ladder_ modBits nLen n a acc bBits b
+
+
+val lemma_bit_xor_is_sum_mod2: a:uint64 -> b:uint64 -> Lemma
+  (requires v a <= 1 /\ v b <= 1)
+  (ensures  v (a ^. b) == (v a + v b) % 2)
+
+let lemma_bit_xor_is_sum_mod2 a b =
+  logxor_spec a b;
+  assert_norm (UInt64.logxor 0uL 0uL == 0uL);
+  assert_norm (UInt64.logxor 0uL 1uL == 1uL);
+  assert_norm (UInt64.logxor 1uL 0uL == 1uL);
+  assert_norm (UInt64.logxor 1uL 1uL == 0uL)
+
+
+val bn_mod_exp_mont_ladder_f_lemma:
+    #nLen:size_nat{nLen + nLen <= max_size_t}
+  -> n:lbignum nLen
+  -> mu:uint64
+  -> bBits:size_pos
+  -> bLen:size_nat{bLen == blocks bBits 64}
+  -> b:lbignum bLen
+  -> i:nat{i < bBits}
+  -> rM0_rM1_sw: tuple3 (lbignum nLen) (lbignum nLen) uint64 -> Lemma
+  (requires
+   (let (rM0, rM1, sw) = rM0_rM1_sw in
+    (1 + (bn_v n % pow2 64) * v mu) % pow2 64 == 0 /\
+    bn_v n % 2 = 1 /\ 1 < bn_v n /\ bn_v n < pow2 (64 * nLen) /\
+    0 < bn_v b /\ bn_v b < pow2 bBits /\
+    bn_v rM0 < bn_v n /\ bn_v rM1 < bn_v n /\ v sw <= 1))
+  (ensures
+   (let (rM0, rM1, sw) = rM0_rM1_sw in
+    let (rM0', rM1', sw') = bn_mod_exp_mont_ladder_f #nLen n mu bBits bLen b i (rM0, rM1, sw) in
+    let (rM0'', rM1'', sw'') = BL.mod_exp_mont_ladder_swap_f_ll nLen (bn_v n) (v mu) bBits (bn_v b) i (bn_v rM0, bn_v rM1, v sw) in
+    bn_v rM0' == rM0'' /\ bn_v rM1' == rM1'' /\ v sw' == sw'' /\
+    bn_v rM0' < bn_v n /\ bn_v rM1' < bn_v n /\ v sw' <= 1))
+
+let bn_mod_exp_mont_ladder_f_lemma #nLen n mu bBits bLen b i (rM0, rM1, sw) =
+  let (rM0', rM1', sw') = bn_mod_exp_mont_ladder_f #nLen n mu bBits bLen b i (rM0, rM1, sw) in
+  let (rM0'', rM1'', sw'') = BL.mod_exp_mont_ladder_swap_f_ll nLen (bn_v n) (v mu) bBits (bn_v b) i (bn_v rM0, bn_v rM1, v sw) in
+  let bit = bn_get_ith_bit #bLen b (bBits - i - 1) in
+  bn_get_ith_bit_lemma #bLen b (bBits - i - 1);
+  //assert (v bit == bn_v b / pow2 (bBits - i - 1) % 2);
+  let sw1 = bit ^. sw in
+  lemma_bit_xor_is_sum_mod2 bit sw;
+  let rM2, rM3 = L.cswap2 sw1 rM0 rM1 in
+  L.cswap2_lemma sw1 rM0 rM1;
+  let rM2' = mont_sqr n mu rM2 in
+  mont_sqr_lemma #nLen n mu rM2;
+  let rM3' = mont_mul n mu rM3 rM2 in
+  mont_mul_lemma #nLen n mu rM3 rM2;
+  assert (rM0' == rM2' /\ rM1' == rM3' /\ sw' == bit);
+  assert (bn_v rM0' == rM0'' /\ bn_v rM1' == rM1'' /\ v sw' == sw'')
+
+
+val bn_mod_exp_mont_ladder_loop_lemma:
+    #nLen:size_nat{nLen + nLen <= max_size_t}
+  -> n:lbignum nLen
+  -> mu:uint64
+  -> bBits:size_pos
+  -> bLen:size_nat{bLen == blocks bBits 64}
+  -> b:lbignum bLen
+  -> i:size_nat{i <= bBits}
+  -> rM0_rM1_sw: tuple3 (lbignum nLen) (lbignum nLen) uint64 -> Lemma
+  (requires
+   (let (rM0, rM1, sw) = rM0_rM1_sw in
+    (1 + (bn_v n % pow2 64) * v mu) % pow2 64 == 0 /\
+    bn_v n % 2 = 1 /\ 1 < bn_v n /\ bn_v n < pow2 (64 * nLen) /\
+    0 < bn_v b /\ bn_v b < pow2 bBits /\
+    bn_v rM0 < bn_v n /\ bn_v rM1 < bn_v n /\ v sw <= 1))
+  (ensures
+   (let (rM0, rM1, sw) = rM0_rM1_sw in
+    let (rM0', rM1', sw') = repeati i (bn_mod_exp_mont_ladder_f #nLen n mu bBits bLen b) (rM0, rM1, sw) in
+    let (rM0'', rM1'', sw'') = repeati i (BL.mod_exp_mont_ladder_swap_f_ll nLen (bn_v n) (v mu) bBits (bn_v b)) (bn_v rM0, bn_v rM1, v sw) in
+    bn_v rM0' == rM0'' /\ bn_v rM1' == rM1'' /\ v sw' == sw'' /\
+    bn_v rM0' < bn_v n /\ bn_v rM1' < bn_v n /\ v sw' <= 1))
+
+let rec bn_mod_exp_mont_ladder_loop_lemma #nLen n mu bBits bLen b i (rM0, rM1, sw) =
+  let (rM0', rM1', sw') = repeati i (bn_mod_exp_mont_ladder_f #nLen n mu bBits bLen b) (rM0, rM1, sw) in
+  let (rM0'', rM1'', sw'') = repeati i (BL.mod_exp_mont_ladder_swap_f_ll nLen (bn_v n) (v mu) bBits (bn_v b)) (bn_v rM0, bn_v rM1, v sw) in
+
+  if i = 0 then begin
+    eq_repeati0 i (bn_mod_exp_mont_ladder_f #nLen n mu bBits bLen b) (rM0, rM1, sw);
+    eq_repeati0 i (BL.mod_exp_mont_ladder_swap_f_ll nLen (bn_v n) (v mu) bBits (bn_v b)) (bn_v rM0, bn_v rM1, v sw);
+    () end
+  else begin
+    unfold_repeati i (bn_mod_exp_mont_ladder_f #nLen n mu bBits bLen b) (rM0, rM1, sw) (i - 1);
+    unfold_repeati i (BL.mod_exp_mont_ladder_swap_f_ll nLen (bn_v n) (v mu) bBits (bn_v b)) (bn_v rM0, bn_v rM1, v sw) (i - 1);
+
+    let (rM2', rM3', sw1') = repeati (i - 1) (bn_mod_exp_mont_ladder_f #nLen n mu bBits bLen b) (rM0, rM1, sw) in
+    let (rM2'', rM3'', sw1'') = repeati (i - 1) (BL.mod_exp_mont_ladder_swap_f_ll nLen (bn_v n) (v mu) bBits (bn_v b)) (bn_v rM0, bn_v rM1, v sw) in
+    assert ((rM0', rM1', sw') == bn_mod_exp_mont_ladder_f #nLen n mu bBits bLen b (i - 1) (rM2', rM3', sw1'));
+    assert ((rM0'', rM1'', sw'') == BL.mod_exp_mont_ladder_swap_f_ll nLen (bn_v n) (v mu) bBits (bn_v b) (i - 1) (rM2'', rM3'', sw1''));
+    bn_mod_exp_mont_ladder_loop_lemma #nLen n mu bBits bLen b (i - 1) (rM0, rM1, sw);
+    assert (bn_v rM2' == rM2'' /\ bn_v rM3' == rM3'' /\ v sw1' == sw1'');
+    bn_mod_exp_mont_ladder_f_lemma #nLen n mu bBits bLen b (i - 1) (rM2', rM3', sw1');
+    () end
+
+
+val bn_mod_exp_mont_ladder_lemma_aux:
+    modBits:size_pos
+  -> nLen:size_pos{nLen = blocks modBits 64 /\ 128 * nLen <= max_size_t}
+  -> n:lbignum nLen
+  -> a:lbignum nLen
+  -> bBits:size_pos
+  -> b:lbignum (blocks bBits 64) -> Lemma
+  (requires
+    bn_v n % 2 = 1 /\ 1 < bn_v n /\ bn_v n < pow2 (64 * nLen) /\
+    0 < bn_v b /\ bn_v b < pow2 bBits /\ bn_v a < bn_v n /\ pow2 (modBits - 1) < bn_v n)
+  (ensures
+   (let mu = mod_inv_u64 n.[0] in
+    let res1 = bn_mod_exp_mont_ladder modBits nLen n a bBits b in
+    let res2 = BL.mod_exp_mont_ladder_swap_ll nLen (bn_v n) (v mu) (bn_v a) bBits (bn_v b) in
+    bn_v res1 == res2 /\ bn_v res1 < bn_v n))
+
+let bn_mod_exp_mont_ladder_lemma_aux modBits nLen n a bBits b =
+  let bLen = blocks bBits 64 in
+
+  let one = bn_from_uint nLen (u64 1) in
+  bn_from_uint_lemma nLen (u64 1);
+  assert (bn_v one == 1);
+
+  let mu = mod_inv_u64 n.[0] in
+  bn_eval_index n 0;
+  assert (bn_v n % pow2 64 == v n.[0]);
+  Math.Lemmas.pow2_modulo_modulo_lemma_1 (bn_v n) 2 64;
+  assert (v n.[0] % 2 = 1); // since bn_v n % 2 = 1
+  mod_inv_u64_lemma n.[0];
+
+  let r2 = precomp_r2_mod_n modBits n in
+  precomp_r2_mod_n_lemma modBits n;
+
+  let rM0 = to_mont #nLen n mu r2 one in
+  to_mont_lemma #nLen n mu r2 one;
+
+  let rM1 = to_mont #nLen n mu r2 a in
+  to_mont_lemma #nLen n mu r2 a;
+
+  let sw = u64 0 in
+  let (rM0', rM1', sw') = repeati bBits (bn_mod_exp_mont_ladder_f #nLen n mu bBits bLen b) (rM0, rM1, sw) in
+  bn_mod_exp_mont_ladder_loop_lemma #nLen n mu bBits bLen b bBits (rM0, rM1, sw);
+
+  let (rM0'', rM1'') = L.cswap2 sw' rM0' rM1' in
+  L.cswap2_lemma sw' rM0' rM1';
+  let res = from_mont n mu rM0'' in
+  from_mont_lemma #nLen n mu rM0''
+
+
+let bn_mod_exp_mont_ladder_lemma modBits nLen n a bBits b =
+  let mu = mod_inv_u64 n.[0] in
+  let r2 = precomp_r2_mod_n modBits n in
+  let res1 = bn_mod_exp_mont_ladder modBits nLen n a bBits b in
+  let res2 = BL.mod_exp_mont_ladder_swap_ll nLen (bn_v n) (v mu) (bn_v a) bBits (bn_v b) in
+  bn_mod_exp_mont_ladder_lemma_aux modBits nLen n a bBits b;
+  assert (bn_v res1 == res2 /\ bn_v res1 < bn_v n);
+
+  bn_eval_index n 0;
+  assert (bn_v n % pow2 64 == v n.[0]);
+  Math.Lemmas.pow2_modulo_modulo_lemma_1 (bn_v n) 2 64;
+  assert (v n.[0] % 2 = 1); // since bn_v n % 2 = 1
+  mod_inv_u64_lemma n.[0];
+  assert ((1 + (bn_v n % pow2 64) * v mu) % pow2 64 == 0);
+
+  let d, k = M.eea_pow2_odd (64 * nLen) (bn_v n) in
+  M.mont_preconditions nLen (bn_v n) (v mu);
+  BL.mod_exp_mont_ladder_swap_ll_lemma nLen (bn_v n) d (v mu) (bn_v a) bBits (bn_v b)
