code/bignum/Hacl.Spec.Bignum.Exponentiation.fsti
@@ -10,9 +10,10 @@ open Hacl.Spec.Bignum.Definitions
 
 #reset-options "--z3rlimit 50 --fuel 0 --ifuel 0"
 
+// This functions is *NOT* constant-time on the exponent b
 val bn_mod_exp:
     modBits:size_pos
-  -> nLen:size_pos{nLen = (blocks modBits 64) /\ 128 * nLen <= max_size_t}
+  -> nLen:size_pos{nLen = blocks modBits 64 /\ 128 * nLen <= max_size_t}
   -> n:lbignum nLen
   -> a:lbignum nLen
   -> bBits:size_pos
@@ -22,7 +23,7 @@ val bn_mod_exp:
 
 val bn_mod_exp_lemma:
     modBits:size_pos
-  -> nLen:size_pos{nLen = (blocks modBits 64) /\ 128 * nLen <= max_size_t}
+  -> nLen:size_pos{nLen = blocks modBits 64 /\ 128 * nLen <= max_size_t}
   -> n:lbignum nLen
   -> a:lbignum nLen
   -> bBits:size_pos
@@ -33,3 +34,29 @@ val bn_mod_exp_lemma:
     pow2 (modBits - 1) < bn_v n) //needed for precomp_r2_mod_n
   (ensures
     bn_v (bn_mod_exp modBits nLen n a bBits b) == Lib.NatMod.pow_mod #(bn_v n) (bn_v a) (bn_v b))
+
+
+// This functions is constant-time on the exponent b
+val bn_mod_exp_mont_ladder:
+    modBits:size_pos
+  -> nLen:size_pos{nLen = blocks modBits 64 /\ 128 * nLen <= max_size_t}
+  -> n:lbignum nLen
+  -> a:lbignum nLen
+  -> bBits:size_pos
+  -> b:lbignum (blocks bBits 64) ->
+  lbignum nLen
+
+
+val bn_mod_exp_mont_ladder_lemma:
+    modBits:size_pos
+  -> nLen:size_pos{nLen = blocks modBits 64 /\ 128 * nLen <= max_size_t}
+  -> n:lbignum nLen
+  -> a:lbignum nLen
+  -> bBits:size_pos
+  -> b:lbignum (blocks bBits 64) -> Lemma
+  (requires
+    bn_v n % 2 = 1 /\ 1 < bn_v n /\ bn_v n < pow2 (64 * nLen) /\
+    0 < bn_v b /\ bn_v b < pow2 bBits /\ bn_v a < bn_v n /\
+    pow2 (modBits - 1) < bn_v n) //needed for precomp_r2_mod_n
+  (ensures
+    bn_v (bn_mod_exp_mont_ladder modBits nLen n a bBits b) == Lib.NatMod.pow_mod #(bn_v n) (bn_v a) (bn_v b))
